Filesys/PathSpec.s.dfy
@@ -18,47 +18,15 @@ module PathSpec {
   import SeqComparison
   import opened SequencesLite
 
-  // equivalent to inode number
-  datatype ID = Nonexistent | ID(id: nat)
-
   type PathElement = seq<byte>
   type Path = seq<PathElement>
-  type PathMap = imap<Path, ID>
 
   const RootDir : Path := [];
-  const RootID := ID(0);
-
-  // robj says: aren't paths all of length >= 1?  Maybe use a subset type or defin a ValidPath predicate?
-  // jialin: we can represent rootdir as empty path
-
-  // jonh: or make Path a datatype and make this a datatype predicate .Complete! (But then you have the extra
-  // syntax that comes with a datatype. :v/ )
-  // jialin: there isn't many pathmap level operations, wrapping in a datatype might make accessing it 
-  //  in the filesystem longer/messier
-  predicate PathMapComplete(path_map: PathMap)
-  {
-    && (forall path :: path in path_map)
-  }
-
-  // robj: Can this be a const?
-  // jonh: what's a const? Isn't this a const?
-  // jialin: imap comprehensions can't be used to define a const
-  //   const is considered as a non-ghost contexts and must be compilable
-  function InitPathMap(): (path_map: PathMap)
-  {
-    imap path :: if path == RootDir then RootID else Nonexistent
-  }
 
   predicate BeneathDir(dir: Path, path: Path)
   {
     && |dir| < |path|
     && path[..|dir|] == dir
-  }
-
-  predicate IsEmptyDir(path_map: PathMap, dir: Path)
-  requires PathMapComplete(path_map)
-  {
-    && (forall k | BeneathDir(dir, k) :: path_map[k].Nonexistent?)
   }
 
   predicate IsDirEntry(dir: Path, path: Path)
